Is0/Wheels.lean
@@ -2,12 +2,22 @@ import Mathlib.Data.Vector.Basic
 
 namespace Option
 
+@[simp]
+lemma get!_of_some {α : Type} [Inhabited α] (x : α) : (some x).get! = x := rfl
+
 end Option
+
+namespace List
+
+def push {α : Type} (x : α) (l : List α) : List α :=
+  l ++ [x]
+
+end List
 
 namespace Vector
 
 def push {α : Type} {k : ℕ} (x : α) : Vector α k → Vector α (k + 1)
-  | ⟨l, h⟩ => ⟨l ++ [x], by simp [h]⟩
+  | ⟨l, h⟩ => ⟨l.push x, by simp [List.push, h]⟩
 
 end Vector
 
